verify vec_index_uniq

theories/typing/lib/vec.v
@@ -77,20 +77,18 @@ Section vec.
   Qed.
   Next Obligation.
     iIntros (????[|d] tid ?? q ?) "LFT In vec κ //=".
-    iDestruct "vec" as (??? aπl[->->]) "(↦tys & ex & †)". iIntros "!>!>!>".
-    rewrite split_big_sepL_mt_ty_own. iDestruct "↦tys" as (?) "[↦ tys]".
-    iMod (ty_own_proph_big_sepL_v with "LFT In tys κ") as "Upd"; [done|].
+    iDestruct "vec" as (??? aπl [->->]) "(↦tys & ex & †)". iIntros "!>!>!>".
+    iMod (ty_own_proph_big_sepL_mt with "LFT In ↦tys κ") as "Upd"; [done|].
     iApply (step_fupdN_wand with "Upd"). iIntros "!> >(%&%&%& ξl & Totys) !>".
     iExists _, _. iSplit.
     { iPureIntro. rewrite -vec_to_list_apply. by apply proph_dep_constr. }
     iIntros "{$ξl}ξl". iMod ("Totys" with "ξl") as "[tys $]". iModIntro.
-    iExists _, _, _, _. iFrame "ex †". iSplit; [done|]. iNext.
-    rewrite split_big_sepL_mt_ty_own. iExists _. iFrame.
+    iExists _, _, _, _. by iFrame.
   Qed.
   Next Obligation.
     iIntros (????[|d] κ ? l' κ' q ?) "LFT In In' vec κ' //=".
     iDestruct "vec" as (?? l aπl ->) "[? tys]". iIntros "!>!>!>".
-    iMod (ty_shr_proph_big_sepL_v with "LFT In In' tys κ'") as "Totys"; [done|].
+    iMod (ty_shr_proph_big_sepL with "LFT In In' tys κ'") as "Totys"; [done|].
     iIntros "!>!>". iApply (step_fupdN_wand with "Totys").
     iIntros ">(%&%&%& ξl & Totys) !>". iExists _, _. iSplit.
     { iPureIntro. rewrite -vec_to_list_apply. by apply proph_dep_constr. }
@@ -119,7 +117,7 @@ Section vec.
   Proof.
     iIntros (Lk ? q ?[|]???) "#LFT #PROPH #E L vec //=".
     iDestruct "vec" as (?? l aπl[->->]) "[↦tys _]". iIntros "!>!>!>".
-    rewrite split_big_sepL_mt_ty_own. iDestruct "↦tys" as (?) "[↦ tys]".
+    rewrite trans_big_sepL_mt_ty_own. iDestruct "↦tys" as (?) "[↦ tys]".
     iMod (leak_big_sepL_ty_own with "LFT PROPH E L tys") as "Upd"; [done..|].
     iApply (step_fupdN_wand with "Upd"). by iIntros "!> ?".
   Qed.
@@ -133,12 +131,12 @@ Section vec.
   Proof.
     move=> Rl. split; iIntros (???[|]) "*% LFT E L vec //=".
     - iDestruct "vec" as (????[->->]) "(↦tys & ex & †)". iIntros "!>!>!>".
-      rewrite split_big_sepL_mt_ty_own. iDestruct "↦tys" as (?) "[↦ tys]".
+      rewrite trans_big_sepL_mt_ty_own. iDestruct "↦tys" as (?) "[↦ tys]".
       iMod (real_big_sepL_ty_own with "LFT E L tys") as "Upd"; [done..|].
       iApply (step_fupdN_wand with "Upd"). iIntros "!> >(%Eq &$&?) !>".
       iSplit; last first.
       { iExists _, _, _, _. iFrame "ex †". iSplit; [done|]. iNext.
-        rewrite split_big_sepL_mt_ty_own. iExists _. iFrame. }
+        rewrite trans_big_sepL_mt_ty_own. iExists _. iFrame. }
       iPureIntro. move: Eq=> [bl Eq]. exists bl. fun_ext=>/= π.
       move: (equal_f Eq π)=>/= <-. by rewrite -vec_to_list_apply vec_to_list_map.
     - iDestruct "vec" as (????->) "[Bor tys]". iIntros "!>!>!>".
@@ -158,7 +156,7 @@ Section vec.
     { move=> ?. elim; [done|]=> ??? IH. fun_ext=>/= ?. f_equal. apply (equal_f IH). }
     do 2 (iSplit; [done|]). iSplit; iIntros "!>" (?[|]) "* vec //=".
     - iDestruct "vec" as (????[->->]) "(↦tys & ex & †)". iExists _, _, _, _.
-      rewrite !split_big_sepL_mt_ty_own Eq EqSz. iSplit; [done|]. iFrame "ex †".
+      rewrite !trans_big_sepL_mt_ty_own Eq EqSz. iSplit; [done|]. iFrame "ex †".
       iNext. iDestruct "↦tys" as (?) "[↦ ?]". iExists _. iFrame "↦".
       by iApply incl_big_sepL_ty_own.
     - iDestruct "vec" as (????->) "[↦ ?]". iExists _, _, _, _. rewrite Eq.
@@ -211,7 +209,7 @@ Section vec.
     case d; [by iDestruct "bvec" as "[>[] _]"|]=> ?.
     iDestruct "bvec" as "[(%&%&%& big) †]".
     iMod (bi.later_exist_except_0 with "big") as (?) "(>-> & >↦₀ & >↦₁ & >↦₂ & big)".
-    wp_read. wp_op. wp_read. do 3 wp_op. wp_read. rewrite split_big_sepL_mt_ty_own.
+    wp_read. wp_op. wp_read. do 3 wp_op. wp_read. rewrite trans_big_sepL_mt_ty_own.
     iDestruct "big" as "((%& ↦old & tys) & (%& %Eq & ↦ex) & †')".
     iDestruct (big_sepL_ty_own_length with "tys") as %Eq'.
     wp_bind (delete _). iApply (wp_delete _ _ _ (_ ++ _) with "[↦old ↦ex †']").
@@ -232,7 +230,7 @@ Section vec.
     iExists _. iFrame "↦". by rewrite unit_ty_own.
   Qed.
 
-  Definition vec_index_shr {𝔄} (ty: type 𝔄) : val :=
+  Definition vec_index {𝔄} (ty: type 𝔄) : val :=
     fn: ["v"; "i"] :=
       letalloc: "r" <- !(!"v" +ₗ #2) +ₗ !"i" * #ty.(ty_size) in
       delete [ #1; "v"];; delete [ #1; "i"];;
@@ -240,7 +238,7 @@ Section vec.
 
   (* The precondition requires that the index is within bounds of the list *)
   Lemma vec_index_shr_type {𝔄} (ty: type 𝔄) :
-    typed_val (vec_index_shr ty) (fn<α>(∅; &shr{α} (vec_ty ty), int) → &shr{α} ty)
+    typed_val (vec_index ty) (fn<α>(∅; &shr{α} (vec_ty ty), int) → &shr{α} ty)
       (λ post '-[al; z], ∃(i: nat) (a: 𝔄), z = i ∧ al !! i = Some a ∧ post a).
   Proof.
     eapply type_fn; [solve_typing|]=> α ??[v[i[]]]. simpl_subst.
@@ -264,16 +262,104 @@ Section vec.
     iApply (wp_delete with "[$↦i $†i]"); [done|]. iIntros "!> _". do 3 wp_seq.
     iMod (proph_obs_sat with "PROPH Obs") as %(?& inat &?&->& Lkup &_); [done|].
     move: Lkup. rewrite -vec_to_list_apply -vlookup_lookup'. move=> [In _].
-    set ifin := nat_to_fin In. have iEq: inat = ifin by rewrite fin_to_nat_to_fin.
+    set ifin := nat_to_fin In. have Eqi: inat = ifin by rewrite fin_to_nat_to_fin.
     rewrite cctx_interp_singleton.
     iApply ("C" $! [# #_] -[aπl !!! ifin] with "Na L [-] []").
     - iSplit; [|done]. rewrite tctx_hasty_val. iExists (S (S d)).
       iSplit. { iApply persistent_time_receipt_mono; [|done]. lia. }
       rewrite/= freeable_sz_full. iFrame "†r". iNext. iExists [_].
       rewrite heap_mapsto_vec_singleton. iFrame "↦r".
-      rewrite/= -Nat2Z.inj_mul iEq. iApply (big_sepL_vlookup with "tys").
+      rewrite/= -Nat2Z.inj_mul Eqi. iApply (big_sepL_vlookup with "tys").
     - iApply proph_obs_impl; [|done]=>/= ?[?[?[/Nat2Z.inj <-[++]]]].
-      by rewrite iEq -vlookup_lookup -vapply_lookup=> <-.
+      by rewrite Eqi -vlookup_lookup -vapply_lookup=> <-.
+  Qed.
+
+  (* The precondition requires that the index is within bounds of the list *)
+  Lemma vec_index_uniq_type {𝔄} (ty: type 𝔄) :
+    typed_val (vec_index ty) (fn<α>(∅; &uniq{α} (vec_ty ty), int) → &uniq{α} ty)
+      (λ post '-[(al, al'); z], ∃(i: nat) (a: 𝔄), z = i ∧
+        al !! i = Some a ∧ ∀a': 𝔄, al' = <[i := a']> al → post (a, a')).
+  Proof.
+    eapply type_fn; [solve_typing|]=> α ??[v[i[]]]. simpl_subst.
+    iIntros (?(vπ &?&[])?) "#LFT #TIME #PROPH UNIQ E Na L C (v & i & _) #Obs".
+    rewrite !tctx_hasty_val.
+    iDestruct "v" as ([|d]) "[#⧖ v]"=>//. case v as [[|v|]|]=>//=.
+    iDestruct "i" as ([|]) "[_ i]"=>//. case i as [[|i|]|]=>//=.
+    wp_bind (new _). iApply wp_new; [done..|]. iIntros "!>% [†r ↦r]".
+    iDestruct "v" as "[(%vl & ↦v & #In & uniq) †v]". case vl as [|[[]|][]]=>//=.
+    iDestruct "i" as "[(%& ↦i & (%&->&->)) †i]". rewrite !heap_mapsto_vec_singleton.
+    iDestruct "uniq" as (d' ξi [Le Eq2]) "[Vo Bor]". set ξ := PrVar _ ξi.
+    iMod (lctx_lft_alive_tok α with "E L") as
+      (?) "((α & α₊ & α₊₊) & L & ToL)"; [solve_typing..|].
+    iMod (bor_acc_cons with "LFT Bor α") as "[(%&%& ↦vec &_& Pc) ToBor]"; [done|].
+    wp_let. iDestruct (uniq_agree with "Vo Pc") as %[<-<-].
+    rewrite split_vec_mt. case d' as [|d']; [done|].
+    iDestruct "↦vec" as (??? aπl Eq1) "(↦₀ & ↦₁ & ↦₂ & ↦tys & ex & †)".
+    have ->: vπ = λ π, (lapply aπl π: list _, π ξ).
+    { rewrite [vπ]surjective_pairing_fun. by rewrite Eq1 Eq2. }
+    wp_read. wp_op. wp_read. wp_read. do 2 wp_op. wp_write.
+    do 2 rewrite -{1}heap_mapsto_vec_singleton. rewrite !freeable_sz_full.
+    wp_bind (delete _). iApply (wp_delete with "[$↦v $†v]"); [done|].
+    iIntros "!>_". wp_seq. wp_bind (delete _).
+    iApply (wp_cumulative_time_receipt with "TIME"); [done|].
+    iApply (wp_delete with "[$↦i $†i]"); [done|]. iIntros "!>_ ⧗". wp_seq.
+    iMod (proph_obs_sat with "PROPH Obs") as %(?& Obs); [done|].
+    move: Obs=> [inat[?[->[+ _]]]]. rewrite -vec_to_list_apply -vlookup_lookup'.
+    move=> [In _]. rewrite -Nat2Z.inj_mul. set ifin := nat_to_fin In.
+    have Eqi: inat = ifin by rewrite fin_to_nat_to_fin.
+    set Inh: Inhabited 𝔄 := populate ((aπl !!! ifin) inhabitant).
+    iDestruct (big_sepL_vtakemiddrop ifin with "↦tys") as "(↦tys & ↦ty & ↦tys')".
+    iMod (ty_own_proph_big_sepL_mt with "LFT In ↦tys α₊") as "Upd"; [done|].
+    setoid_rewrite shift_loc_ty_assoc.
+    iMod (ty_own_proph_big_sepL_mt with "LFT In ↦tys' α₊₊") as "Upd'"; [done|].
+    iCombine "Upd Upd'" as "Upd". rewrite fupd_sep. wp_bind Skip.
+    iApply (wp_step_fupdN_persistent_time_receipt _ _ ∅ with "TIME ⧖ [Upd]");
+      [done|done| |].
+    { iApply step_fupdN_with_emp. rewrite difference_empty_L.
+      iApply step_fupdN_nmono; [|iApply "Upd"]. lia. }
+    wp_seq. iIntros "[(%ξl &%&%& ξl & To↦tys) (%ξl' &%&%& ξl' & To↦tys')] !>". wp_seq.
+    iMod (uniq_intro (aπl !!! ifin) with "PROPH UNIQ") as (ζi) "[Vo' Pc']"; [done|].
+    set ζ := PrVar _ ζi. iDestruct (uniq_proph_tok with "Vo' Pc'") as "(Vo' & ζ & Pc')".
+    rewrite proph_tok_singleton.
+    iDestruct (proph_tok_combine with "ζ ξl'") as (?) "[ζξl Toζξl]".
+    iDestruct (proph_tok_combine with "ξl ζξl") as (?) "[ξζξl Toξζξl]".
+    iMod (uniq_preresolve ξ _ (lapply (vinsert ifin (.$ ζ) aπl))
+      with "PROPH Vo Pc ξζξl") as "(Obs' & ξζξl & ToPc)"; [done| |].
+    { rewrite -vec_to_list_apply.
+      apply proph_dep_constr, proph_dep_vinsert=>//. apply proph_dep_one. }
+    iCombine "Obs Obs'" as "#?". iClear "Obs".
+    iDestruct ("Toξζξl" with "ξζξl") as "[ξl ζξl]".
+    iDestruct ("Toζξl" with "ζξl") as "[ζ ξl']". iSpecialize ("Pc'" with "ζ").
+    iMod ("To↦tys" with "ξl") as "(↦tys & α₊)".
+    iMod ("To↦tys'" with "ξl'") as "(↦tys' & α₊₊)".
+    iMod ("ToBor" with "[⧗ ↦₀ ↦₁ ↦₂ ex † ↦tys ↦tys' ToPc] [↦ty Pc']")
+      as "[Bor α]"; last first.
+    - rewrite cctx_interp_singleton.
+      iMod ("ToL" with "[$α $α₊ $α₊₊] L") as "L".
+      iApply ("C" $! [# #_] -[λ π, ((aπl !!! ifin) π, π ζ)] with "Na L [-] []").
+      + iSplitL; [|done]. rewrite tctx_hasty_val. iExists _.
+        rewrite -freeable_sz_full. iFrame "⧖ †r". iNext. iExists [_].
+        rewrite heap_mapsto_vec_singleton. iFrame "↦r In". iExists d', _.
+        iFrame "Vo' Bor". iPureIntro. split; [lia|done].
+      + iApply proph_obs_impl; [|done]=>/= ?[[?[?[/Nat2Z.inj <-[++]]]]Eqξ].
+        rewrite Eqi -vlookup_lookup=> <- Imp. rewrite -vapply_lookup. apply Imp.
+        by rewrite Eqξ -vec_to_list_apply vapply_insert -vec_to_list_insert.
+    - iNext. iExists _, _. rewrite -Eqi. iFrame "↦ty Pc'".
+      iApply persistent_time_receipt_mono; [|done]. lia.
+    - iIntros "!> (%&%& ↦ty & >⧖' & Pc)". iCombine "⧖ ⧖'" as "⧖!".
+      iMod (cumulative_persistent_time_receipt with "TIME ⧗ ⧖!")
+        as "⧖!"; [solve_ndisj|]. iIntros "/=!>!>".
+      iExists _, _. iFrame "⧖!". iDestruct ("ToPc" with "[Pc]") as "$".
+      { iDestruct (proph_ctrl_eqz with "PROPH Pc") as "Eqz".
+        rewrite -vec_to_list_apply. iApply proph_eqz_constr.
+        by iApply proph_eqz_vinsert. }
+      rewrite split_vec_mt. iExists _, _, _, _. iFrame "↦₀ ↦₁ ↦₂ ex †".
+      iSplit; [by rewrite vec_to_list_apply|]. iNext. iClear "#".
+      rewrite vinsert_backmid -big_sepL_vbackmid Eqi. iSplitL "↦tys".
+      { iStopProof. do 6 f_equiv. iApply ty_own_depth_mono. lia. }
+      iSplitL "↦ty". { iStopProof. do 3 f_equiv. iApply ty_own_depth_mono. lia. }
+      iStopProof. do 6 f_equiv; [|iApply ty_own_depth_mono; lia].
+      f_equiv. rewrite shift_loc_assoc_nat. f_equal. lia.
   Qed.
 
   Definition vec_push {𝔄} (ty: type 𝔄) : val :=
@@ -365,7 +451,7 @@ Section vec.
     wp_op. wp_write. wp_op. wp_read. wp_let. do 3 wp_op. wp_bind (new _).
     iApply wp_new; [lia|done|]. iIntros "!>" (?) "[†' ↦']". wp_let. wp_op.
     have ->: ∀sz: nat, ((2 * len + 1) * sz)%Z = (len + S len) * sz by lia.
-    rewrite split_big_sepL_mt_ty_own plus_0_r Nat2Z.id Nat.mul_add_distr_r
+    rewrite trans_big_sepL_mt_ty_own plus_0_r Nat2Z.id Nat.mul_add_distr_r
       repeat_app heap_mapsto_vec_app.
     iDestruct "↦tys" as (?) "[↦ tys]". iDestruct "↦'" as "[↦' ↦ex']".
     iDestruct (big_sepL_ty_own_length with "tys") as %Len. wp_bind (memcpy _).
@@ -373,7 +459,7 @@ Section vec.
     iIntros "!>[↦' ↦]". wp_seq. wp_op. rewrite -Nat2Z.inj_mul. wp_bind (delete _).
     iApply (wp_delete with "[$↦ †]"); [lia|by rewrite Len|]. iIntros "!>_".
     wp_seq. wp_op. wp_write. iApply "push". iExists _, _. iFrame "↦₀ ↦₁ ↦₂".
-    iSplitL "↦' tys". { rewrite split_big_sepL_mt_ty_own. iExists _. iFrame. }
+    iSplitL "↦' tys". { rewrite trans_big_sepL_mt_ty_own. iExists _. iFrame. }
     iSplitR "†'".
     - iExists _. rewrite repeat_length. iFrame "↦ex'". by rewrite repeat_length.
     - by have <-: ∀sz, sz + (len + len) * sz = len * sz + (sz + len * sz) by lia.
@@ -396,7 +482,7 @@ Section vec.
       letalloc: "r" <-{ty.(ty_size)} ! !("v'" +ₗ #2) +ₗ "len'" * #ty.(ty_size) in
       return: ["r"].
 
-  (* The precondition requires that the input list has a positive length *)
+  (* The precondition requires that the input list is non-empty *)
   Lemma vec_pop_type {𝔄} (ty: type 𝔄) :
     typed_val (vec_pop ty) (fn<α>(∅; &uniq{α} (vec_ty ty)) → ty)
       (λ post '-[(al, al')],
@@ -410,8 +496,7 @@ Section vec.
     rewrite heap_mapsto_vec_singleton. wp_read. wp_let. wp_bind (delete _).
     rewrite -heap_mapsto_vec_singleton freeable_sz_full.
     iApply (wp_delete with "[$↦ $†]"); [done|]. iIntros "!>_".
-    iDestruct "uniq" as (d i [? Eq2]) "[Vo Bor]".
-    move: Eq2. set ξ := PrVar _ i=> Eq2.
+    iDestruct "uniq" as (d i [? Eq2]) "[Vo Bor]". move: Eq2. set ξ := PrVar _ i=> Eq2.
     iMod (lctx_lft_alive_tok α with "E L") as (?) "(α & L & ToL)"; [solve_typing..|].
     iMod (bor_acc with "LFT Bor α") as "[(%&%& ↦vec & #⧖ & Pc) ToBor]"; [done|].
     wp_seq. iDestruct (uniq_agree with "Vo Pc") as %[<-<-].
